---
layout: post
title: ูุณุงุฆู ูุญูููุฉ ูู ุงููุนุงุฏูุงุช ุงูุชุฑุจูุนูุฉ
tag: ุฌุจุฑ
---

## ๐ ุงููุธุฑูุฉ ุงูุฃุณุงุณูุฉ

**ุงููุนุงุฏูุฉ ุงูุชุฑุจูุนูุฉ ุงูุนุงูุฉ:**
$$ax^2 + bx + c = 0 \quad (a \neq 0)$$

**ุงููููุฒ:** 
$\Delta = b^2 - 4ac$

**ุตูุบุฉ ุงูุญููู:**
$$x = \frac{-b \pm \sqrt{b^2 - 4ac}}{2a}$$

- ุฅุฐุง ูุงู $\Delta > 0$: ุญูุงู ุญููููุงู ูุฎุชููุงู
- ุฅุฐุง ูุงู $\Delta = 0$: ุญู ูุงุญุฏ ูุถุงุนู
- ุฅุฐุง ูุงู $\Delta < 0$: ุญูุงู ุนูุฏูุงู

---

## ๐ ูุซุงู ูก
ุฃูุฌุฏ ุญููู ุงููุนุงุฏูุฉ
$$x^2 - 5x + 6 = 0$$

<details>
  <summary>ุงููุฑ ููุง ูุฑุคูุฉ ุงูุญู</summary>
  
<strong>ุงูุทุฑููุฉ ุงูุฃููู (ุงูุชุญููู):</strong>

$$x^2 - 5x + 6 = (x-2)(x-3) = 0$$
$$x = 2 \text{ ุฃู } x = 3$$

</strong>ุงูุทุฑููุฉ ุงูุซุงููุฉ (ุงููุงููู ุงูุนุงู):</strong>
$$a=1, b=-5, c=6$$

$$\Delta = (-5)^2 - 4(1)(6) = 25 - 24 = 1$$

$$x = \frac{5 \pm \sqrt{1}}{2} = \frac{5 \pm 1}{2}$$

$$x = 3 \text{ ุฃู } x = 2$$

</details>
